Paranoia v4

theories/Paranoia.v
@@ -3,286 +3,731 @@ From Equations Require Import Equations.
 From LogRel.AutoSubst Require Import core unscoped Ast Extra.
 From LogRel Require Import Utils Context Weakening.
 
+From Ltac2 Require Import Ltac2 Printf.
+(* From Ltac2 Require Control Constr List Ltac1 Std Notations. *)
+
 Unset Automatic Proposition Inductives.
+Set Default Goal Selector "all".
 
-Inductive nftykind : Type :=
-  | nfPi
-  | nfNat.
 
+Ltac2 depelim (i : ident) : unit := ltac1:(i |- depelim i) (Ltac1.of_ident i).
+Ltac2 Notation "depelim" i(ident) := depelim i.
+
+Ltac2 noconf (i : ident) : unit := ltac1:(i |- noconf i) (Ltac1.of_ident i).
+Ltac2 Notation "noconf" i(ident) := noconf i.
+
+Ltac2 eassumption0 := fun () => ltac1:(eassumption).
+Ltac2 Notation "eassumption" := eassumption0 ().
+
+Ltac2 Notation ">" c(thunk(tactic)) := Control.enter c.
+Ltac2 Notation c1(thunk(self)) "+" c2(thunk(tactic)) := Control.plus c1 (fun _ => c2 ()).
+Ltac2 Notation c1(thunk(self)) "||" c2(thunk(tactic)) := Notations.orelse c1 (fun _ => c2 ()).
+Ltac2 Notation "[>" tacs(list0(thunk(self),"|")) "]" := Control.dispatch tacs.
+
+Ltac2 Notation "only" startgoal(tactic) endgoal(opt(seq("-", tactic))) ":" tac(thunk(tactic)) :=
+  Control.focus startgoal (Option.default startgoal endgoal) tac.
+
+Inductive renames (Γ : context) : forall (ρ : nat -> nat) (Δ : context), Type :=
+  | ren_empty {ρ} :
+      renames Γ ρ ε
+  | ren_tm {Δ A ρ} :
+      renames Γ (↑ >> ρ) Δ
+   -> in_ctx Γ (ρ 0) A⟨↑ >> ρ⟩
+   -> renames Γ ρ (Δ ,, A).
+
+Scheme renames_rect_nodep := Minimality for renames Sort Type.
+Derive Signature for renames.
+
+Lemma VarRen {Γ A n}
+  (H : in_ctx Γ n A)
+  : forall {Δ τ}
+  (X : renames Δ τ Γ),
+  in_ctx Δ (τ n) A⟨τ⟩.
+Proof.
+  induction H. intros **.
+  depelim X.
+  rewrite -> !renRen_term.
+  ltac1:(change (τ (S ?n)) with ((↑ >> τ) n)).
+  eauto.
+Defined.
+
+Lemma RenComp {Γ Δ ρ}
+  (H : renames Γ ρ Δ)
+  : forall {Ξ τ}
+  (X : renames Ξ τ Γ),
+  renames Ξ (ρ >> τ) Δ.
+Proof.
+  induction H.
+  intros **.
+  econstructor.
+  - eauto.
+  - change (↑ >> (ρ >> τ)) with ((↑ >> ρ) >> τ).
+    rewrite <- !(renRen_term (↑ >> ρ)).
+    change ((ρ >> τ) 0) with (τ (ρ 0)).
+    eapply VarRen.
+    eassumption.
+Defined.
+
+Fixpoint iter {A} (n : nat) (f : A -> A) : A -> A :=
+  match n with
+  | O => id
+  | S n => iter n f >> f
+  end.
+
+Lemma iter_inside {A} (n : nat) (f : A -> A)
+  : iter (S n) f = f >> iter n f.
+Proof.
+  revert f.
+  induction n.
+  - reflexivity.
+  - intros ?.
+    cbn delta [iter] iota.
+    ltac1:(change ((?a >> ?b) >> ?c) with (a >> (b >> c))).
+    apply (f_equal (fun g => g >> f)).
+    apply IHn.
+Defined.
+
+Lemma VarWk {Γ A n}
+  (H : in_ctx Γ n A) :
+  forall {T},
+  in_ctx (Γ ,,, T) (iter #|T| ↑ n) A⟨iter #|T| ↑⟩.
+Proof.
+  induction H.
+  intros T.
+  induction T.
+  cbn.
+  rewrite -> ?rinstId'_term, <- ?renRen_term.
+  econstructor; eauto.
+Defined.
+
+Lemma RenWeakening {Γ Ξ ρ}
+  (H : renames Γ ρ Ξ) :
+  forall T,
+  renames (Γ ,,, T) (ρ >> iter #|T| ↑) Ξ.
+Proof.
+  induction H.
+  econstructor.
+  ltac1:(change (↑ >> (iter #|T| ↑ >> ρ)) with ((↑ >> iter #|T| ↑) >> ρ)).
+  - eapply IHrenames.
+  - change (↑ >> (ρ >> iter #|T| ↑)) with ((↑ >> ρ) >> iter #|T| ↑).
+    rewrite <- renRen_term.
+    eapply VarWk; eassumption.
+Defined.
+
+Lemma RenWeakenOnce {Γ Ξ ρ}
+  (H : renames Γ ρ Ξ) :
+  forall {A},
+  renames (Γ ,, A) (ρ >> ↑) Ξ.
+Proof.
+  intros A.
+  apply (RenWeakening H (ε ,, A)).
+Defined.
+
+(* Type system *)
 Reserved Notation "[ |- Γ ≡ Γ' ]".
 Reserved Notation "[ Γ ≡ Γ' |- A ≡ B ]".
-Reserved Notation "[ Γ ≡ Γ' |- t ≡ t' # A ≡ B ]".
-Reserved Notation "[ Γ ≡ Γ' |- t ≡nf t' '#Π' Dom , Cod ≡ Dom' , Cod' ]".
-Reserved Notation "[ Γ ≡ Γ' |- t ≡nf t' '#Nat' ]".
+Reserved Notation "[ Γ ≡ Γ' |- A ≡whnf B ]".
+Reserved Notation "[ Γ ≡ Γ' |- t ≡ t' ◁ A ≡ B ]".
+Reserved Notation "[ Γ ≡ Γ' |- t ≡whnf t' ▷ A ≡whnf B ]".
+Reserved Notation "[ Γ ≡ Γ' |- t ≡ t' ▷ A ≡whnf B ]".
 Reserved Notation "[ Γ ≡ Γ' |- A ≡ne B ]".
-Reserved Notation "[ Γ ≡ Γ' |- t ≡ne t' # A ≡ B ]".
+Reserved Notation "[ Γ ≡ Γ' |- t ≡ne t' '▷red' A ≡ B ]".
+Reserved Notation "[ Γ ≡ Γ' |- t ≡ne t' ▷ A ≡ B ]".
 Reserved Notation "[ Γ |- A ~> B ]".
 Reserved Notation "[ Γ |- A ~* B ]".
+Reserved Notation "[ Γ |- t ↗ u ]".
 Reserved Notation "[ Γ |- t ~>tm u ]".
 Reserved Notation "[ Γ |- t ~*tm u ]".
 
-Unset Elimination Schemes.
-
-Inductive ConvCont : context -> context -> Type :=
+Inductive ConvCont : forall (Γ Γ' : context), Type :=
   | connil :
       [ |- ε ≡ ε ]
   | concons {Γ Γ' A B} :
       [ Γ ≡ Γ' |- A ≡ B]
    -> [ |- Γ ,, A ≡ Γ' ,, B]
-with ConvTy : forall (_ _ : context) (_ _ : term), Type :=
-  | tyNat {Γ Γ' A B} :
+with ConvTy : forall (Γ Γ' : context) (A B : term), Type :=
+  | normTy {Γ Γ' A B A' B'} :
+      [ Γ ≡ Γ' |- A' ≡whnf B' ]
+   -> [ Γ |- A ~* A' ]
+   -> [ Γ' |- B ~* B' ]
+   -> [ Γ ≡ Γ' |- A ≡ B ]
+with ConvWhnfTy : forall (Γ Γ' : context) (A B : term), Type :=
+  | nfNat {Γ Γ'} :
       [ |- Γ ≡ Γ' ]
-   -> [ Γ |- A ~* tNat ]
-   -> [ Γ' |- B ~* tNat ]
-   -> [ Γ ≡ Γ' |- A ≡ B ]
-  | tyProd {Γ Γ' A B Dom Dom' Cod Cod'} :
-      [ Γ |- A ~* tProd Dom Cod ]
-   -> [ Γ' |- B ~* tProd Dom' Cod' ]
-   -> [ Γ ≡ Γ' |- Dom ≡ Dom' ]
-   -> [ Γ ,, Dom ≡ Γ' ,, Dom' |- Cod ≡ Cod' ]
-   -> [ Γ ≡ Γ' |- A ≡ B ]
-with ConvNeTy : forall (_ _ : context) (_ _ : term), Type :=
-with ConvNfProd : forall (_ _ : context) (_ _ _ _ : term) (_ _ : term), Type :=
-  | nfFun {Γ Γ' Dom Dom' Cod Cod' t t'} :
+   -> [ Γ ≡ Γ' |- tNat ≡whnf tNat ]
+  | nfProd {Γ Γ' Dom Dom' Cod Cod'} :
       [ Γ ≡ Γ' |- Dom ≡ Dom' ]
    -> [ Γ ,, Dom ≡ Γ' ,, Dom' |- Cod ≡ Cod' ]
-   -> [ Γ ,, Dom ≡ Γ' ,, Dom' |- tApp (t ⟨↑⟩) (tRel 0) ≡ tApp (t' ⟨↑⟩) (tRel 0) # Cod ≡ Cod' ]
-   -> [ Γ ≡ Γ' |- t ≡nf t' #Π Dom , Cod ≡ Dom' , Cod' ]
-with ConvNfNat : forall (_ _ : context) (_ _ : term), Type :=
-  | tmZero {Γ Γ' t t'} :
+   -> [ Γ ≡ Γ' |- tProd Dom Cod ≡whnf tProd Dom' Cod' ]
+with ConvNeTy : forall (Γ Γ' : context) (A B : term), Type :=
+with ConvCheckTm : forall (Γ Γ' : context) (A B : term) (t u : term), Type :=
+  | check {Γ Γ' A B A' B' t t'} :
+      [ Γ ≡ Γ' |- t ≡ t' ▷ A ≡whnf B ]
+   -> [ Γ ≡ Γ |- A' ≡ A ]
+   -> [ Γ' ≡ Γ' |- B' ≡ B ]
+   -> [ Γ ≡ Γ' |- t ≡ t' ◁ A' ≡ B' ]
+with ConvTm : forall (Γ Γ' : context) (A B : term) (t u : term), Type :=
+  | norm {Γ Γ' A B t t' u u'} :
+      [ Γ ≡ Γ' |- t ≡whnf t' ▷ A ≡whnf B ]
+   -> [ Γ |- u ~*tm t ]
+   -> [ Γ' |- u' ~*tm t' ]
+   -> [ Γ ≡ Γ' |- u ≡ u' ▷ A ≡whnf B ]
+with ConvWhnfTm : forall (Γ Γ' : context) (A B : term) (t u : term), Type :=
+  | nfZero {Γ Γ'} :
       [ |- Γ ≡ Γ' ]
-   -> [ Γ |- t ~* tZero ]
-   -> [ Γ' |- t' ~* tZero ]
-   -> [ Γ ≡ Γ' |- t ≡nf t' #Nat ]
-  | tmSucc {Γ Γ' t t' u u'} :
-      [ Γ |- t ~* tSucc u ]
-   -> [ Γ' |- t' ~* tSucc u' ]
-   -> [ Γ ≡ Γ' |- u ≡nf u' #Nat ]
-   -> [ Γ ≡ Γ' |- t ≡nf t' #Nat ]
-  | tmNeNat {Γ Γ' A B t t' n n'} :
-      [ Γ |- A ~* tNat ]
-   -> [ Γ' |- B ~* tNat ]
-   -> [ Γ |- t ~* n ]
-   -> [ Γ' |- t' ~* n' ]
-   -> [ Γ ≡ Γ' |- n ≡ne n' # A ≡ B ]
-   -> [ Γ ≡ Γ' |- t ≡nf t' #Nat ]
-with ConvTm : forall (_ _ : context) (_ _ : term) (_ _ : term), Type :=
-  | tmNat {Γ Γ' A B t t'} :
-      [ Γ |- A ~* tNat ]
-   -> [ Γ' |- B ~* tNat ]
-   -> [ Γ ≡ Γ' |- t ≡nf t' #Nat ]
-   -> [ Γ ≡ Γ' |- t ≡ t' # A ≡ B ]
-  | tmPi {Γ Γ' A B Dom Dom' Cod Cod' t t'} :
-      [ Γ |- A ~* tProd Dom Cod ]
-   -> [ Γ' |- B ~* tProd Dom' Cod' ]
-   -> [ Γ ≡ Γ' |- t ≡nf t' #Π Dom , Cod ≡ Dom' , Cod' ]
-   -> [ Γ ≡ Γ' |- t ≡ t' # A ≡ B ]
-with ConvNeTm : forall (_ _ : context) (_ _ : term) (_ _ : term), Type :=
-  | tmNeVar {Γ Γ' A B n} :
+   -> [ Γ ≡ Γ' |- tZero ≡whnf tZero ▷ tNat ≡whnf tNat ]
+  | nfSucc {Γ Γ' t t'} :
+      [ Γ ≡ Γ' |- t ≡ t' ▷ tNat ≡whnf tNat ]
+   -> [ Γ ≡ Γ' |- tSucc t ≡whnf tSucc t' ▷ tNat ≡whnf tNat ]
+  | nfNeNat {Γ Γ' n n'} :
+      [ Γ ≡ Γ' |- n ≡ne n' ▷red tNat ≡ tNat ]
+   -> [ Γ ≡ Γ' |- n ≡whnf n' ▷ tNat ≡whnf tNat ]
+  | nfLambda {Γ Γ' Dom Dom' Cod Cod' t t'} :
+      [ Γ ≡ Γ' |- Dom ≡ Dom' ]
+   -> [ Γ ,, Dom ≡ Γ' ,, Dom' |- t ≡ t' ▷ Cod ≡whnf Cod' ]
+   -> [ Γ ≡ Γ' |- tLambda Dom t ≡whnf tLambda Dom' t' ▷ tProd Dom Cod ≡whnf tProd Dom' Cod' ]
+with ConvNeRedTm : forall (Γ Γ' : context) (A B : term) (t u : term), Type :=
+  | tyReduces {Γ Γ' n n' A B A' B'} :
+      [ Γ ≡ Γ' |- n ≡ne n' ▷ A ≡ B ]
+   -> [ Γ |- A ~* A' ]
+   -> [ Γ' |- B ~* B' ]
+   -> [ Γ ≡ Γ' |- n ≡ne n' ▷red A' ≡ B' ]
+with ConvNeTm : forall (Γ Γ' : context) (A B : term) (t u : term), Type :=
+  | neVar {Γ Γ' A B n} :
       [ |- Γ ≡ Γ' ]
    -> in_ctx Γ n A
    -> in_ctx Γ' n B
-   -> [ Γ ≡ Γ' |- tRel n ≡ne tRel n # A ≡ B ]
-  | tmNeApp {Γ Γ' A B Dom Dom' Cod Cod' t t' u u'} :
-      [ Γ ≡ Γ' |- t ≡ne t' # A ≡ B ]
-   -> [ Γ |- A ~* tProd Dom Cod ]
-   -> [ Γ' |- B ~* tProd Dom' Cod' ]
+   -> [ Γ ≡ Γ' |- tRel n ≡ne tRel n ▷ A ≡ B ]
+  | neApp {Γ Γ' Dom Dom' Cod Cod' t t' u u'} :
+      [ Γ ≡ Γ' |- t ≡ne t' ▷red tProd Dom Cod ≡ tProd Dom' Cod' ]
    -> [ Γ ≡ Γ' |- Dom ≡ Dom' ]
+   -> [ Γ ≡ Γ' |- u ≡ u' ◁ Dom ≡ Dom' ]
    -> [ Γ ,, Dom ≡ Γ' ,, Dom' |- Cod ≡ Cod' ]
-   -> [ Γ ≡ Γ' |- u ≡ u' # Dom ≡ Dom' ]
    -> [ Γ ≡ Γ' |- Cod[u..] ≡ Cod'[u'..] ]
-   -> [ Γ ≡ Γ' |- tApp t u  ≡ne tApp t' u' # Cod[u..] ≡ Cod'[u'..] ]
-with RedTyStep : forall (_ : context) (_ _ : term), Type :=
-with RedTy : forall (_ : context) (_ _ : term), Type :=
+   -> [ Γ ≡ Γ' |- tApp t u ≡ne tApp t' u' ▷ Cod[u..] ≡ Cod'[u'..] ]
+  | neNatElim {Γ Γ' P P' hz hz' hs hs' t t'} :
+      [ Γ ,, tNat ≡ Γ' ,, tNat |- P ≡ P' ]
+   -> [ Γ ≡ Γ' |- hz ≡ hz' ◁ P[tZero..] ≡ P'[tZero..] ]
+   -> [ Γ ≡ Γ' |- hs ≡ hs' ◁ tProd tNat P[(tSucc (tRel 0))]⇑ ≡ tProd tNat P'[(tSucc (tRel 0))]⇑ ]
+   -> [ Γ ≡ Γ' |- t ≡ne t' ▷red tNat ≡ tNat ]
+   -> [ Γ ≡ Γ' |- P[t..] ≡ P'[t'..] ]
+   -> [ Γ ≡ Γ' |- tNatElim P hz hs t ≡ne tNatElim P' hz' hs' t' ▷ P[t..] ≡ P'[t'..] ]
+(* with RedTyStep : forall (Γ : context) (A B : term), Type := *)
+with RedTy : forall (Γ : context) (A B : term), Type :=
   | redTyDone {Γ A} :
-      [ Γ |- A ~* A ]
-  | redTyStep {Γ A B C} :
-      [ Γ |- A ~> B ]
-   -> [ Γ |- B ~* C ]
-   -> [ Γ |- A ~* C ]
-with RedTmStep : forall (_ : context) (_ _ : term), Type :=
+      [ |- Γ ≡ Γ]
+   -> [ Γ |- A ~* A ]
+  (* | redTyStep {Γ A B C} :
+   *     [ Γ |- A ~> B ]
+   *  -> [ Γ |- B ~* C ]
+   *  -> [ Γ |- A ~* C ] *)
+with RedTmStep : forall (Γ : context) (t u : term), Type :=
   | redBeta {Γ A B t u} :
       [ Γ ≡ Γ |- A ≡ A ]
-   -> [ Γ ,, A ≡ Γ ,, A |- B ≡ B ]
-   -> [ Γ ,, A ≡ Γ ,, A |- t ≡ t # B ≡ B ]
-   -> [ Γ ≡ Γ |- u ≡ u # A ≡ A ]
+   -> [ Γ ,, A ≡ Γ ,, A |- t ≡ t ▷ B ≡whnf B ]
+   -> [ Γ ≡ Γ |- u ≡ u ▷ A ≡whnf A ]
    -> [ Γ |- tApp (tLambda A t) u ~>tm t[u..] ]
-  | redAppHead {Γ A B t t' u} :
-      [ Γ ≡ Γ |- A ≡ A ]
-   -> [ Γ ,, A ≡ Γ ,, A |- B ≡ B ]
-   -> [ Γ ≡ Γ |- t' ≡ t' # tProd A B ≡ tProd A B ]
-   -> [ Γ |- t ~>tm t' ]
+  | redAppHead {Γ t t' u} :
+      [ Γ |- t ~>tm t' ]
    -> [ Γ |- tApp t u ~>tm tApp t' u ]
-with RedTm : forall (_ : context) (_ _ : term), Type :=
-  | redTmDone {Γ t} :
-      [ Γ |- t ~*tm t ]
+with ExpTmStep : forall (Γ : context) (t u : term), Type :=
+  | expandPi {Γ n Dom Cod} :
+      [ Γ ≡ Γ |- n ≡ne n ▷red tProd Dom Cod ≡ tProd Dom Cod ]
+   -> [ Γ |- n ↗ tLambda Dom (tApp n⟨↑⟩ (tRel 0)) ]
+with RedTm : forall (Γ : context) (t u : term), Type :=
+  | redTmNoEta {Γ t} :
+      [ |- Γ ≡ Γ]
+   -> [ Γ |- t ~*tm t ]
+  | redTmEta {Γ t u} :
+      [ |- Γ ≡ Γ]
+   -> [ Γ |- t ↗ u ]
+   -> [ Γ |- t ~*tm u ]
   | redTmStep {Γ t t' t''} :
       [ Γ |- t ~>tm t' ]
    -> [ Γ |- t' ~*tm t'' ]
    -> [ Γ |- t ~*tm t'' ]
   where "[ |- Γ ≡ Γ' ]" := (ConvCont Γ Γ')
     and "[ Γ ≡ Γ' |- A ≡ B ]" := (ConvTy Γ Γ' A B)
-    and "[ Γ ≡ Γ' |- t ≡ t' # A ≡ B ]" := (ConvTm Γ Γ' A B t t')
-    and "[ Γ ≡ Γ' |- t ≡nf t' '#Π' Dom , Cod ≡ Dom' , Cod' ]" := (ConvNfProd Γ Γ' Dom Cod Dom' Cod' t t')
-    and "[ Γ ≡ Γ' |- t ≡nf t' '#Nat' ]" := (ConvNfNat Γ Γ' t t')
+    and "[ Γ ≡ Γ' |- A ≡whnf B ]" := (ConvWhnfTy Γ Γ' A B)
+    and "[ Γ ≡ Γ' |- t ≡ t' ◁ A ≡ B ]" := (ConvCheckTm Γ Γ' A B t t')
+    and "[ Γ ≡ Γ' |- t ≡ t' ▷ A ≡whnf B ]" := (ConvTm Γ Γ' A B t t')
+    and "[ Γ ≡ Γ' |- t ≡whnf t' ▷ A ≡whnf B ]" := (ConvWhnfTm Γ Γ' A B t t')
     and "[ Γ ≡ Γ' |- A ≡ne B ]" := (ConvNeTy Γ Γ' A B)
-    and "[ Γ ≡ Γ' |- t ≡ne t' # A ≡ B ]" := (ConvNeTm Γ Γ' A B t t')
-    and "[ Γ |- A ~> B ]" := (RedTyStep Γ A B)
+    and "[ Γ ≡ Γ' |- t ≡ne t' '▷red' A ≡ B ]" := (ConvNeRedTm Γ Γ' A B t t')
+    and "[ Γ ≡ Γ' |- t ≡ne t' ▷ A ≡ B ]" := (ConvNeTm Γ Γ' A B t t')
+    (* and "[ Γ |- A ~> B ]" := (RedTyStep Γ A B) *)
     and "[ Γ |- A ~* B ]" := (RedTy Γ A B)
+    and "[ Γ |- t ↗ u ]" := (ExpTmStep Γ t u)
     and "[ Γ |- t ~>tm u ]" := (RedTmStep Γ t u)
     and "[ Γ |- t ~*tm u ]" := (RedTm Γ t u).
 
-(* Maybe try with a specific conversion relation at each whnf type *)
-(* Also separate reduction and conversion more cleanly *)
+Derive NoConfusion for term.
 
-Derive Signature for ConvCont.
-Derive Signature for ConvTy.
-Derive Signature for ConvTm.
-Derive Signature for ConvNfNat.
-Derive Signature for ConvNfProd.
-Derive Signature for ConvNeTm.
-Derive Signature for RedTy.
-Derive Signature for RedTyStep.
-Derive Signature for RedTmStep.
-Derive Signature for RedTm.
+Derive Signature for ConvCont
+ConvTy
+ConvWhnfTy
+ConvCheckTm
+ConvTm
+ConvWhnfTm
+ConvNeRedTm
+ConvNeTm
+RedTy
+(* RedTyStep *)
+RedTmStep
+ExpTmStep
+RedTm.
 
 Scheme ConvCont_rect_nodep := Minimality for ConvCont Sort Type
   with ConvTy_rect_nodep := Minimality for ConvTy Sort Type
+  with ConvWhnfTy_rect_nodep := Minimality for ConvWhnfTy Sort Type
+  with ConvCheckTm_rect_nodep := Minimality for ConvCheckTm Sort Type
   with ConvTm_rect_nodep := Minimality for ConvTm Sort Type
-  with ConvNfNat_rect_nodep := Minimality for ConvNfNat Sort Type
-  with ConvNfProd_rect_nodep := Minimality for ConvNfProd Sort Type
+  with ConvWhnfTm_rect_nodep := Minimality for ConvWhnfTm Sort Type
+  with ConvNeRedTm_rect_nodep := Minimality for ConvNeRedTm Sort Type
   with ConvNeTm_rect_nodep := Minimality for ConvNeTm Sort Type
   with RedTy_rect_nodep := Minimality for RedTy Sort Type
+  (* with RedTyStep_rect_nodep := Minimality for RedTyStep Sort Type *)
   with RedTmStep_rect_nodep := Minimality for RedTmStep Sort Type
+  with ExpTmStep_rect_nodep := Minimality for ExpTmStep Sort Type
   with RedTm_rect_nodep := Minimality for RedTm Sort Type.
 
 Combined Scheme _Syntax_rect_nodep from
 ConvCont_rect_nodep,
 ConvTy_rect_nodep,
+ConvWhnfTy_rect_nodep,
+ConvCheckTm_rect_nodep,
 ConvTm_rect_nodep,
-ConvNfNat_rect_nodep,
-ConvNfProd_rect_nodep,
+ConvWhnfTm_rect_nodep,
+ConvNeRedTm_rect_nodep,
 ConvNeTm_rect_nodep,
 RedTy_rect_nodep,
 RedTmStep_rect_nodep,
+ExpTmStep_rect_nodep,
 RedTm_rect_nodep.
 
+Ltac2 make_forall (x : ident) (dom : constr) (body : constr -> constr) : constr :=
+  let f := Constr.in_context x dom (fun () => let body := body (Control.hyp x) in exact $body) in
+  match Constr.Unsafe.kind f with
+    | Constr.Unsafe.Lambda f cl => Constr.Unsafe.make (Constr.Unsafe.Prod f cl)
+    | _ => Control.throw Assertion_failure
+  end.
+
+
+Ltac2 make_fun (x : ident) (dom : constr) (body : constr -> constr) : constr :=
+  Constr.in_context x dom (fun () => let body := body (Control.hyp x) in exact $body).
+
+Ltac2 get_binder (body : constr) : ident option :=
+  match Constr.Unsafe.kind body with
+    | Constr.Unsafe.Prod f _ => Constr.Binder.name f
+    | Constr.Unsafe.Lambda f _ => Constr.Binder.name f
+    | _ => None
+  end.
+
+Ltac2 in_goal_opt (x : ident option) : ident :=
+  match x with
+  | Some x => Fresh.in_goal x
+  | None => Fresh.in_goal @x
+  end.
+
+Ltac2 rec polymorphise t :=
+  lazy_match! t with
+    | forall x : ?hyp, @?t x => make_forall (in_goal_opt (get_binder t)) hyp
+      (fun x => let t' := eval hnf in ($t $x) in let t'' := polymorphise t' in t'')
+    | (?t1 * ?t2)%type => let t1' := polymorphise t1 in let t2' := polymorphise t2 in
+        constr:($t1' × $t2')
+    | ?t' => t'
+  end.
+
+Ltac2 rec remove_steps t :=
+  lazy_match! t with
+  | _ -> ?t => remove_steps t
+  | forall x : ?dom, @?t x => make_fun (in_goal_opt (get_binder t)) dom
+      (fun x => let t' := eval hnf in ($t $x) in let t'' := remove_steps t' in t'')
+  | ?t' => t'
+  end.
+
 Definition _SyntaxInductionType :=
-  ltac:(let ind := fresh "ind" in
+  ltac2:(let ind := Fresh.in_goal @ind in
       pose (ind := _Syntax_rect_nodep);
-      refold ;
-      let ind_ty := type of ind in
-      exact ind_ty).
+      fold ind ;
+      let ind_ty := Constr.type (Control.hyp ind) in
+      exact $ind_ty).
 
 Definition SyntaxInductionType :=
-  ltac: (let ind := eval cbv delta [_SyntaxInductionType] zeta
+  ltac2: (let ind := eval cbv delta [_SyntaxInductionType] zeta
     in _SyntaxInductionType in
     let ind' := polymorphise ind in
-  exact ind').
+  exact $ind').
 
 Definition SyntaxInduction : SyntaxInductionType.
 Proof.
-  intros P1 P2 P3 P4 P5 P6 P7 P8 P9 **.
-  assert (H : _) by (apply (_Syntax_rect_nodep P1 P2 P3 P4 P5 P6 P7 P8 P9); assumption).
-  repeat econstructor; apply H.
+  intros ?**.
+  let h :=
+    List.fold_left
+      (fun a (b,_,_) => let b := Control.hyp b in constr:($a $b))
+      constr:(_Syntax_rect_nodep)
+      (Control.hyps ())
+  in pose (H := $h).
+  repeat split.
+  apply H.
 Defined.
 
-Definition SyntaxInductionConcl := ltac:(let t := eval cbv delta [SyntaxInductionType] beta in SyntaxInductionType in let t' := remove_steps t in exact t').
+Definition SyntaxInductionConcl := ltac2:(let t := eval cbv delta [SyntaxInductionType] beta in SyntaxInductionType in let t' := remove_steps t in exact $t').
 Print SyntaxInductionConcl.
 
-Lemma Conv_ConvCont : SyntaxInductionConcl
-  (fun _ _ => unit)
-  (fun Γ Γ' _ _ => [ |- Γ ≡ Γ' ])
-  (fun Γ Γ' _ _ _ _ => [ |- Γ ≡ Γ' ])
-  (fun Γ Γ' _ _ => [ |- Γ ≡ Γ' ])
-  (fun Γ Γ' _ _ _ _ _ _ => [ |- Γ ≡ Γ' ])
-  (fun Γ Γ' _ _ _ _ => [ |- Γ ≡ Γ' ])
-  (fun Γ _ _ => unit)
-  (fun Γ _ _ => unit)
-  (fun Γ _ _ => unit).
+(* TODO: Should be in Constr? *)
+(* Substitutes the argument in the body of a given lambda *)
+Ltac2 app_lambda (lam : constr) (a : constr) : constr :=
+  match Constr.Unsafe.kind lam with
+  | Constr.Unsafe.Lambda _ body => Constr.Unsafe.substnl [a] 0 body
+  | _ => Control.throw Assertion_failure
+  end.
+
+Ltac2 decompose_app_list (c : constr) :=
+  match Constr.Unsafe.kind c with
+    | Constr.Unsafe.App f cl => (f, Array.to_list cl)
+    | _ => (c,[])
+  end.
+
+Ltac2 mkApp_list (h : constr) (args : constr list) : constr :=
+  match args with
+  | [] => h
+  | _ => Constr.Unsafe.make (Constr.Unsafe.App h (Array.of_list args))
+  end.
+
+Ltac2 syntax_ind_concl (f : constr -> constr) :=
+  let rec transform_clause t :=
+    lazy_match! t with
+    (* XXX: Need to give a name to _cod so that it only matches closed terms *)
+    | ?dom -> ?_cod =>
+      let r := f dom in constr:($dom -> $r)
+    | forall (x : ?dom), @?a x => make_forall (in_goal_opt (get_binder t)) dom
+        (fun x => transform_clause (app_lambda a x))
+    end
+  in
+  let rec transform_clauses t :=
+    lazy_match! t with
+    | fun (x : ?dom) => @?a x =>
+      let f := make_fun (in_goal_opt (get_binder t)) dom
+        (fun x => transform_clauses (app_lambda a x))
+      in
+      lazy_match! f with
+      | fun _ => ?b => b
+      end
+    | ?a × ?b => let a := transform_clause a in let b := transform_clauses b in constr:($a × $b)
+    | ?a => let a := transform_clause a in a
+    end in
+  let t := eval cbv [SyntaxInductionConcl] in SyntaxInductionConcl in
+  let res := transform_clauses t in
+  res.
+
+Ltac2 Notation "syntax_ind_concl" t(next) := syntax_ind_concl t.
+
+Ltac2 synt_ind_arity (c : constr) :=
+  lazy_match! c with
+  | ConvCont => 2
+  | ConvTy => 2
+  | ConvWhnfTy => 2
+  | ConvCheckTm => 2
+  | ConvTm => 2
+  | ConvWhnfTm => 2
+  | ConvNeRedTm => 2
+  | ConvNeTm => 2
+  | RedTy => 1
+  (* | RedTyStep => 1 *)
+  | RedTmStep => 1
+  | ExpTmStep => 1
+  | RedTm => 1
+  end.
+
+Lemma Conv_ConvCont : ltac2:(
+  let f t :=
+    let (head, args) := decompose_app_list t in
+    match (synt_ind_arity head) with
+    | 2 => let Γ := List.nth args 0 in
+           let Γ' := List.nth args 1 in
+           constr:([ |- $Γ ≡ $Γ' ])
+    | 1 => let Γ := List.nth args 0 in
+           constr:([ |- $Γ ≡ $Γ ])
+    | _ => constr:(unit)
+    end in
+  refine (syntax_ind_concl f)).
 Proof.
-  eapply SyntaxInduction; easy.
+  Print SyntaxInductionType.
+  apply SyntaxInduction.
+  > intros **.
+  > repeat (exact tt || assumption || constructor).
 Defined.
 
-Lemma Conv_Symm : SyntaxInductionConcl
-  (fun Γ Γ' => [ |- Γ' ≡ Γ ])
-  (fun Γ Γ' A B => [ Γ' ≡ Γ |- B ≡ A ])
-  (fun Γ Γ' A B t u => [ Γ' ≡ Γ |- u ≡ t # B ≡ A ])
-  (fun Γ Γ' t u => [ Γ' ≡ Γ |- u ≡nf t #Nat ])
-  (fun Γ Γ' Dom Cod Dom' Cod' t u => [ Γ' ≡ Γ |- u ≡nf t #Π Dom' , Cod' ≡ Dom , Cod ])
-  (fun Γ Γ' A B t u => [ Γ' ≡ Γ |- u ≡ne t # B ≡ A ] )
-  (fun _ _ _ => unit)
-  (fun _ _ _ => unit)
-  (fun _ _ _ => unit).
+Ltac2 fold_righti (f : int -> 'a -> 'b -> 'b) (ls : 'a list) (a : 'b) : 'b :=
+  let rec go i ls a :=
+    match ls with
+    | [] => a
+    | l :: ls => f i l (go (Int.add i 1) ls a)
+    end
+  in go 0 ls a.
+
+Ltac2 unzip (ls : 'a list) : 'a list * 'a list :=
+  let f i x (l, r) :=
+    if Int.equal (Int.mod i 2) 0
+    then (x :: l, r)
+    else (l, x :: r)
+  in
+  fold_righti f ls ([],[]).
+
+Ltac2 rec zipWith (f : 'a -> 'b -> 'c) (l : 'a list) (r : 'b list) : 'c list :=
+  match l with
+  | [] => []
+  | hl :: l =>
+    match r with
+    | [] => []
+    | hr :: r => f hl hr :: zipWith f l r
+  end end.
+
+Ltac2 zip (l : 'a list) (r : 'b list) : ('a * 'b) list :=
+  zipWith (fun a b => (a, b)) l r.
+
+Ltac2 uncurry (f : 'a -> 'b -> 'c) (u : 'a * 'b) : 'c :=
+  let (a , b) := u in f a b.
+
+Lemma Conv_Symm : ltac2:(
+  let f t :=
+    let (head, args) := decompose_app_list t in
+    match (synt_ind_arity head) with
+    | 2 => let m := List.concat (uncurry (zipWith (fun a b => [b ; a])) (unzip args)) in
+        mkApp_list head m
+    | _ => constr:(unit)
+    end in
+  refine (syntax_ind_concl f)).
 Proof.
-  eapply SyntaxInduction; now econstructor.
+  apply SyntaxInduction; now econstructor.
 Defined.
 
-Fixpoint redStepDet {Γ A B C}
-  (H1 : [ Γ |- A ~> B ])
-  (H2 : [ Γ |- A ~> C ])  :
-   B = C.
+Lemma Conv_Left : ltac2:(
+  let f t :=
+    let (head, args) := decompose_app_list t in
+    match (synt_ind_arity head) with
+    | 2 => let m := List.concat (uncurry (zipWith (fun a _ => [a ; a])) (unzip args)) in
+        mkApp_list head m
+    | _ => constr:(unit)
+    end in
+  let t := syntax_ind_concl f
+  in exact $t).
 Proof.
-  depelim H1.
+  apply SyntaxInduction; now econstructor.
 Defined.
 
-Derive NoConfusion for term.
+Ltac2 Notation "rename" renames(list1(seq(ident, "into", ident), ",")) := Std.rename renames.
 
-Fixpoint redTmStepDet {Γ t u u'}
-  (H1 : [ Γ |- t ~>tm u ])
-  (H2 : [ Γ |- t ~>tm u' ])  :
-   u = u'.
+
+Ltac2 rec eapplyprod c :=
+  (Unification.unify (TransparentState.current ()) c open_constr:((_ , _));
+  eapply (fst $c) + eapplyprod constr:(snd $c))
+  + eapply $c.
+
+Ltac2 convsymmetries () :=
+  () + eapply Conv_Left; () + eapply Conv_Symm.
+
+Instance Ren_nat_nat : Ren1 (nat -> nat) nat nat := fun f n => f n.
+
+Lemma substRen {t u ρ} : t[u..]⟨ρ⟩ = t⟨upRen_term_term ρ⟩[u⟨ρ⟩..].
 Proof.
-  depelim H1; depelim H2.
-  - reflexivity.
-  - depelim H2.
-  - depelim H1.
-  - now f_equal.
+  ltac1:(asimpl).
+  reflexivity.
 Defined.
 
-Definition whnfTyb (t : term) := match t with | tProd _ _ => true | tNat => true | _ => false end.
-
-Fixpoint redDet {Γ A B C}
-  (H1 : [ Γ |- A ~* B ])
-  (H2 : [ Γ |- A ~* C ])
-  (Bwhnf : whnfTyb B = true)
-  (Cwhnf : whnfTyb C = true) :
-   B = C.
+Lemma shiftScons {t : term} {n ρ} : t⟨↑⟩⟨n .: ρ⟩ = t⟨ρ⟩.
 Proof.
-  depelim H1; depelim H2.
-  - reflexivity.
-  - depelim A; noconf Bwhnf; depelim r.
-  - depelim A; noconf Cwhnf; depelim r.
-  - assert (H : B = B0) by now eapply redStepDet. subst. now eapply redDet.
+  ltac1:(asimpl).
+  reflexivity.
 Defined.
 
+Lemma substUp {t u ρ} : t⟨upRen_term_term ρ⟩[u⟨upRen_term_term ρ⟩]⇑ = t[u]⇑⟨upRen_term_term ρ⟩.
+Proof.
+  ltac1:(asimpl).
+  reflexivity.
+Defined.
+
+Ltac2 myautosubst_tac () :=
+  cbn delta [ren1 Ren_term ren_term Ren_nat_nat upRen_term_term up_ren scons] beta iota in *;
+  rewrite <- ?shift_upRen, -> ?substRen, -> ?shiftScons in * |- *.
+
+Create HintDb typing discriminated.
+
+Hint Resolve Conv_Left Conv_Symm : typing.
+Hint Constructors ConvCont
+ConvTy
+ConvWhnfTy
+ConvCheckTm
+ConvTm
+ConvWhnfTm
+ConvNeRedTm
+ConvNeTm
+RedTy
+RedTmStep
+ExpTmStep
+RedTm
+
+in_ctx
+renames : typing.
+
+Print HintDb typing.
+
+Ltac2 iter_hypo (f : ident -> unit) := match! goal with [ h : _ |- _] => f h end.
+
+(* Lemmas *)
+Lemma RenStable : ltac2:(
+  let f t :=
+    let (head, args) := decompose_app_list t in
+    match (synt_ind_arity head) with
+    | 2 =>
+      let (Γ , Γ' , args) := match args with
+      | Γ :: (Γ' :: args) => Γ , Γ' , args
+      | _ => Control.throw Assertion_failure
+      end in
+       constr:(forall (Δ Δ' : context) ρ,
+         [ |- Δ ≡ Δ' ] -> renames Δ ρ $Γ -> renames Δ' ρ $Γ' ->
+         ltac2:(refine (mkApp_list head (&Δ :: &Δ' :: (List.map (fun c => constr:($c⟨&ρ⟩)) args)))))
+    | 1 =>
+      let (Γ , args) := match args with
+      | Γ :: args => Γ , args
+      | _ => Control.throw Assertion_failure
+      end in
+      constr:(forall (Δ : context) ρ,
+        [ |- Δ ≡ Δ] -> renames Δ ρ $Γ ->
+        ltac2:(refine (mkApp_list head (&Δ ::(List.map (fun c => constr:($c⟨&ρ⟩)) args)))))
+    | _ => constr:(unit)
+    end in
+  refine (syntax_ind_concl f)).
+Proof.
+  apply SyntaxInduction.
+  > (intros *; repeat (first [ intros ? ? * | try (rename H into H'); intros H ])).
+  1-2: eassumption.
+
+  myautosubst_tac ().
+
+  (* Use resp. each constructor of the mind block  *)
+  let s := Env.get [@LogRel; @Paranoia; @ConvCont] in
+  let ref := match s with | Some (Std.IndRef i) => i | _ => Control.throw Assertion_failure end
+  in
+  let data := Ind.data ref
+  in
+  let instance := match Constr.Unsafe.kind (Env.instantiate (Std.IndRef ref)) with
+    | Constr.Unsafe.Ind _ i => i
+    | _ => Control.throw Assertion_failure end
+  in
+  let blocks := List.map (fun i => Ind.get_block data i) (List.init (Ind.nblocks data) (fun i => i))
+  in
+  let constructors :=
+    List.concat
+      (List.map (fun block => List.map (fun i => Ind.get_constructor block i) (List.init (Ind.nconstructors block) (fun i => i))) blocks)
+  in
+  let constrs := List.map (fun c => Constr.Unsafe.make (Constr.Unsafe.Constructor c instance)) constructors
+  in
+  let tacs := List.map (fun constr () => eapply $constr) constrs
+  in Control.dispatch (List.skipn 2 tacs).
+  > lazy_match! goal with
+    | [ |- in_ctx _ _ _ ] => eauto using VarRen
+    | [ |- _] => ()
+    end.
+
+  try (ltac1:(change (?a ⟨upRen_term_term ρ⟩[?b ..]) with (a ⟨upRen_term_term ρ⟩[b⟨ρ⟩ ..]))).
+  try (ltac1:(change (?a ⟨upRen_term_term ρ⟩[?b]⇑) with (a ⟨upRen_term_term ρ⟩[b⟨upRen_term_term ρ⟩]⇑))).
+  rewrite <- ?substRen, -> ?substUp.
+
+  try (once (repeat (> iter_hypo (fun h => let h := Control.hyp h in eapply $h) || (eapply Conv_Left; now (() + eapply Conv_Symm)) || econstructor || eapply RenWeakenOnce || (ltac1:(change (↑ >> upRen_term_term ?ρ) with (ρ >> ↑)); rewrite <- (renRen_term _ ↑)))); >fail).
+Defined.
+
+Ltac2 bing () := iter_hypo (fun h => let h := Control.hyp h in eapply $h) || (now convsymmetries ()) || econstructor.
+
+Lemma Output : SyntaxInductionConcl
+  (fun Γ Γ' => unit)
+  (fun Γ Γ' A B => unit)
+  (fun Γ Γ' A B => unit)
+  (fun Γ Γ' A B t u => unit)
+  (fun Γ Γ' A B t u => forall Γ'' t' A' C, [ Γ'' ≡ Γ' |- t' ≡ u ▷ A' ≡whnf C ] -> B = C)
+  (fun Γ Γ' A B t u => forall Γ'' t' A' C, [ Γ'' ≡ Γ' |- t' ≡whnf u ▷ A' ≡whnf C ] -> B = C)
+  (fun Γ Γ' A B t u => forall Γ'' t' A' C, [ Γ' ≡ Γ' |- B ≡whnf B ]
+    -> [ Γ' ≡ Γ' |- C ≡whnf C ] -> [ Γ'' ≡ Γ' |- t' ≡ne u ▷red A' ≡ C ] -> B = C)
+  (fun Γ Γ' A B t u => forall Γ'' t' A' C, [ Γ'' ≡ Γ' |- t' ≡ne u ▷ A' ≡ C ] -> B = C)
+  (fun Γ A B => forall C, [ Γ ≡ Γ |- B ≡whnf B ] -> [ Γ ≡ Γ |- C ≡whnf C ] -> [ Γ |- A ~* C ]  -> B = C)
+  (fun Γ t u => forall v, [ Γ |- t ~>tm v ] -> u = v)
+  (fun Γ t u => forall v, [ Γ |- t ↗ v ] -> u = v)
+  (fun Γ t u => forall v A B,
+       [ Γ ≡ Γ |- u ≡whnf u ▷ A ≡whnf A ]
+    -> [ Γ ≡ Γ |- v ≡whnf v ▷ B ≡whnf B ]
+    -> [ Γ |- t ~*tm v ]
+    -> u = v).
+Proof.
+  eapply SyntaxInduction; intros *; repeat (first [ intros ? ? * | try (rename H into H'); intros H ]).
+  all: try (lazy_match! goal with [|- unit] => constructor end).
+  depelim H.
+  (* > iter_hypo (fun h => try (let h' := Control.hyp h in erewrite $h' by bing (); printf "%I" h; clear0 [h])). *)
+   try (once (repeat (> reflexivity || progress f_equal || bing () || iter_hypo (fun h => let h' := Control.hyp h in progress (erewrite ! $h' by bing ())) || eapply in_ctx_inj)); >fail).
+  1: depelim H'; depelim c.
+  1: depelim c; depelim c.
+  1: f_equal.
+  1-2: Control.shelve ().
+  - bing ().
+    depelim H5.
+    erewrite ?H0 by bing ().
+    > bing ().
+    > bing ().
+    > bing ().
+    > bing ().
+  - bing ().
+    erewrite H4 by bing ().
+    bing ().
+  - depelim H'.
+    depelim c.
+    erewrite H4 by bing ().
+    bing ().
+    > bing ().
+    > bing (). depelim H; reflexivity.
+  - depelim H; reflexivity.
+  - depelim H; try reflexivity.
+    depelim X; depelim c.
+  - depelim H.
+    + depelim c; depelim c.
+    + f_equal; tea eapply H0.
+  - depelim X2.
+    assert (__ : B = B0) by (tea eapply H'). subst.
+    tea eapply H1.
+  - depelim H.
+    tea eapply in_ctx_inj.
+  - depelim H.
+    f_equal.
+    enough (prodeq : tProd Dom' Cod' = tProd Dom'0 Cod'0) by (noconf prodeq; reflexivity).
+    eapply H' > [eassumption | ..]; econstructor.
+Defined.
 
 Lemma Conv_Trans : SyntaxInductionConcl
   (fun Γ Γ' => forall Γ'', [ |- Γ' ≡ Γ'' ] -> [ |- Γ ≡ Γ'' ])
   (fun Γ Γ' A B => forall Γ'' C, [ Γ' ≡ Γ'' |- B ≡ C ] -> [ Γ ≡ Γ'' |- A ≡ C ])
-  (fun Γ Γ' A B t u => forall Γ'' C v, [ Γ' ≡ Γ'' |- u ≡ v # B ≡ C ] -> [ Γ ≡ Γ'' |- t ≡ v # A ≡ C ])
-  (fun Γ Γ' t u => forall Γ'' v, [ Γ' ≡ Γ'' |- u ≡nf v #Nat ] -> [ Γ ≡ Γ'' |- t ≡nf v #Nat ])
-  (fun Γ Γ' Dom Cod Dom' Cod' t u => forall Γ'' Dom'' Cod'' v,
-    [ Γ' ≡ Γ'' |- u ≡nf v #Π Dom' , Cod' ≡ Dom'' , Cod'' ]
-    -> [ Γ ≡ Γ'' |- t ≡nf v #Π Dom , Cod ≡ Dom'' , Cod'' ])
-  (fun Γ Γ' A B t u => forall Γ'' C v, [ Γ' ≡ Γ'' |- u ≡ne v # B ≡ C ] -> [ Γ ≡ Γ'' |- t ≡ne v # A ≡ C ] )
+  (fun Γ Γ' A B => forall Γ'' C, [ Γ' ≡ Γ'' |- B ≡whnf C ] -> [ Γ ≡ Γ'' |- A ≡whnf C ])
+  (fun Γ Γ' A B t u => forall Γ'' C v, [ Γ' ≡ Γ'' |- u ≡ v ◁ B ≡ C ] -> [ Γ ≡ Γ'' |- t ≡ v ◁ A ≡ C ])
+  (fun Γ Γ' A B t u => forall Γ'' C v, [ Γ' ≡ Γ'' |- u ≡ v ▷ B ≡whnf C ] -> [ Γ ≡ Γ'' |- t ≡ v ▷ A ≡whnf C ])
+  (fun Γ Γ' A B t u => forall Γ'' C v, [ Γ' ≡ Γ'' |- u ≡whnf v ▷ B ≡whnf C ] -> [ Γ ≡ Γ'' |- t ≡whnf v ▷ A ≡whnf C ])
+  (fun Γ Γ' A B t u => forall Γ'' C v, [ Γ' ≡ Γ'' |- u ≡ne v ▷red B ≡ C ] -> [ Γ ≡ Γ'' |- t ≡ne v ▷red A ≡ C ])
+  (fun Γ Γ' A B t u => forall Γ'' C v, [ Γ' ≡ Γ'' |- u ≡ne v ▷ B ≡ C ] -> [ Γ ≡ Γ'' |- t ≡ne v ▷ A ≡ C ])
+  (fun _ _ _ => unit)
   (fun _ _ _ => unit)
   (fun _ _ _ => unit)
   (fun _ _ _ => unit).
 Proof.
-  eapply SyntaxInduction; intros *; repeat first [ intros ? ? * | try rename H into H'; intros H ].
-  all: try lazymatch goal with [|- unit] => constructor end.
+  eapply SyntaxInduction; intros *; repeat (first [ intros ? ? * | try (rename H into H'); intros H ]).
+  all: try (lazy_match! goal with [|- unit] => constructor end).
   all: depelim H.
   - now econstructor.
   - now econstructor.
   - now econstructor.
-  - assert (conf : tNat = tProd Dom Cod) by (eapply redDet; easy). noconf conf.
-  - eassert (conf : tNat = tProd _ _) by (eapply (redDet (A := A0)); easy).
-    noconf conf.
-  - assert (noconf : tProd Dom' Cod' = tProd Dom0 Cod0) by (eapply redDet; easy).
-    noconf noconf.
-    eapply tyProd; easy.
-  -
+  - invertRedTy.
+  - invertRedTy.
+  - invertRedTy.
+    now eapply tyProd.
+  - econstructor.
+    + eapply X0.
+  - assert ()
 Defined.
 
 Fixpoint ConvTm_ConvTy {Γ Γ' t t' A B}
